NLustre/Stream.v
@@ -77,13 +77,6 @@ if the clocked stream is [absent] at the corresponding instant. *)
   (** ** Synchronous functions *)
 
   (** Count the number of resets ticks seen at [n] so far. *)
-  (* Fixpoint count (rs: cstream) (n: nat) : nat := *)
-  (*   match n, rs n with *)
-  (*   | 0, false => 0 *)
-  (*   | 0, true => 1 *)
-  (*   | S m, false => count rs m *)
-  (*   | S m, true => S (count rs m) *)
-  (*   end. *)
   Fixpoint count (rs: cstream) (n: nat) : nat :=
     let c := match n with 0 => 0 | S n => count rs n end in
     if rs n then S c else c.
@@ -91,11 +84,7 @@ if the clocked stream is [absent] at the corresponding instant. *)
   (** [mask o k rs xs] is the stream which clips the stream [xs] between
       the [k]th and the [(k+1)]th reset, outputting [o] everywhere else. *)
   Definition mask {A} (opaque: A) (k: nat) (rs: cstream) (xs: stream A) : stream A :=
-    fun n =>
-      if beq_nat k (count rs n) then xs n else opaque.
-
-  (* Definition masked {A} (k: nat) (rs: cstream) (xs xs': stream A) := *)
-  (*   forall n, count rs n = k -> xs' n = xs n. *)
+    fun n => if beq_nat k (count rs n) then xs n else opaque.
 
   (** ** Properties *)
 
